return new position instead of writing it in a buffer

steel/formats/everparse/Veritas.Formats.fst
@@ -8,18 +8,16 @@ let serialize_value v dst =
 
 module U64 = FStar.UInt64
 
-let extract_log_entry_from len buf bpos =
+let extract_log_entry_from len buf pos =
   let h = HST.get () in
   let sl = LP.make_slice buf len in
-  let pos = B.index bpos 0ul in
   let pos' = Veritas.Formats.EverParse.Vlog_entry.vlog_entry_validator sl (FStar.Int.Cast.uint32_to_uint64 pos) in
   if LP.is_error pos'
-  then None // raise "extract_log_entry: no valid log entry"
+  then Inr (pos (* FIXME: constrain position in pos' *), "extract_log_entry: no valid log entry")
   else begin
     LP.valid_facts Veritas.Formats.EverParse.Vlog_entry.vlog_entry_parser h sl pos;
-    B.upd bpos 0ul (LP.uint64_to_uint32 pos');
     LP.parse_strong_prefix Veritas.Formats.EverParse.Vlog_entry.vlog_entry_parser (LP.bytes_of_slice_from h sl pos) (B.as_seq h (B.gsub buf pos (LP.uint64_to_uint32 pos' `U32.sub` pos)));
-    Some (Veritas.Formats.EverParse.Vlog_entry.vlog_entry_reader sl pos)
+    Inl (Veritas.Formats.EverParse.Vlog_entry.vlog_entry_reader sl pos, LP.uint64_to_uint32 pos')
   end
 
 let serialize_stamped_record dst r =
